recurrence stub

dp/problems.dfy
@@ -1,12 +1,34 @@
+include "../prop.dfy"
+
 // 6.1
-// (TODO) Recurrence of contiguous subsequence of maxium sum:
-function recContiguousSubsequence(): nat
+// Base case(s):
+predicate sumOfEmptySubseq(subSeq: seq<int>, sum: int) 
 {
-    0
+    |subSeq| == 0 ==> sum == 0
 }
 
-method contiguousSubsequence(a: seq<nat>) returns (b: seq<nat>)
-ensures |b| < |a|
+predicate sumOfSingletonSeq(sequences: seq<int>, sum: int) 
 {
-    assume |b| < |a|;
+    |sequences| == 1 ==> sum == 0
+}
+
+// (TODO) Recurrence of contiguous subsequence of maxium sum:
+function recMaxContiguousSubseq(s: seq<int>, i: int): int
+requires 0 <= i < |s|
+{
+    if i-1 < 0 
+        then 0
+    else
+    if s[i] > s[i] + recMaxContiguousSubseq(s, i-1)
+        then s[i]
+    else s[i] + recMaxContiguousSubseq(s, i-1)
+}
+
+method maxContiguousSubseq(a: seq<int>) returns (subSeq: seq<int>, sum: int)
+ensures Prop.shorterThan(subSeq, a)
+ensures Prop.subsetOf(subSeq, a)
+ensures Prop.increasing(subSeq) // or strictly increasing?
+ensures sumOfEmptySubseq(subSeq, sum)
+ensures sumOfSingletonSeq(a, sum)
+{
 }
